parser/Parser_error_free.v
@@ -20,66 +20,69 @@ Module ParserErrorFreeFn (Import D : Defs.T).
    i.e., impossible states really are impossible *)
 
   Lemma stacks_wf__step_neq_invalid_state :
-    forall (g     : grammar)
-           (pm    : production_map)
+    forall (gr    : grammar)
+           (hw    : grammar_wf gr)
+           (rm    : rhs_map)
            (cm    : closure_map)
-           (ps    : prefix_stack)
-           (ss    : suffix_stack)
+           (sk    : parser_stack)
            (ts    : list token)
            (vi    : NtSet.t)
            (un    : bool)
            (ca    : cache)
-           (hc    : cache_stores_target_results pm cm ca)
-           (hk    : stack_pushes_from_keyset pm ss),
-      stacks_wf g ps ss
-      -> step pm cm ps ss ts vi un ca hc hk <> StepError InvalidState.
+           (hc    : cache_stores_target_results rm cm ca)
+           (hk    : stack_pushes_from_keyset rm sk),
+      stack_wf gr sk
+      -> step gr hw rm cm sk ts vi un ca hc hk <> StepError InvalidState.
   Proof.
-    intros g pm cm ps ss ts vi un ca hc hk hw; unfold not; intros hs. 
-    unfold step in hs; dms; tc; try inv hw.
+    intros gr hw rm cm sk ts vi un ca hc hk hw'; unfold not; intros hs. 
+    unfold step in hs; dmeqs H; tc; rew_anr; inv hw'; rew_anr.
+    eapply fpaa_none_contra; eauto.
   Qed.
 
   Lemma multistep_never_reaches_error_state :
-    forall (g    : grammar)
-           (pm   : production_map)
+    forall (gr   : grammar)
+           (hw   : grammar_wf gr) 
+           (rm   : rhs_map)
+           (hr   : rhs_map_correct rm gr)
            (cm   : closure_map)
+           (x    : nonterminal)
            (tri  : nat * nat * nat)
            (ha   : Acc lex_nat_triple tri)
-           (ps   : prefix_stack)
-           (ss   : suffix_stack)
+           (sk   : parser_stack)
            (ts   : list token)
            (vi   : NtSet.t)
            (un   : bool)
            (ca   : cache)
-           (hc   : cache_stores_target_results pm cm ca)
-           (hk   : stack_pushes_from_keyset pm ss)
-           (ha'  : Acc lex_nat_triple (meas pm ss ts vi)),
-      tri = meas pm ss ts vi
-      -> production_map_correct pm g
-      -> stacks_wf g ps ss
-      -> multistep pm cm ps ss ts vi un ca hc hk ha' <> Error InvalidState.
+           (hc   : cache_stores_target_results rm cm ca)
+           (hk   : stack_pushes_from_keyset rm sk)
+           (hb   : bottom_stack_sym_eq_start_sym sk x)
+           (ha'  : Acc lex_nat_triple (parser_meas rm sk ts vi)),
+      tri = parser_meas rm sk ts vi
+      -> stack_wf gr sk
+      -> multistep gr hw rm hr cm x sk ts vi un ca hc hk hb ha' <> Error _ InvalidState.
   Proof.
-    intros g pm cm tri ha'.
+    intros gr hw rm hr cm x tri ha'.
     induction ha' as [tri hlt IH].
-    intros ps ss ts vi un ca hc hk ha ? hp hw hm; subst. 
+    intros sk ts vi un ca hc hk hb ha ? hw' hm; subst. 
     apply multistep_cases in hm.
     destruct hm as [hs | hm].
     - eapply stacks_wf__step_neq_invalid_state; eauto.
-    - destruct hm as (ps' & ss' & ts' & av' & un' & ca' & hc' & hk' & ha' & hs & hm).
+    - destruct hm as (sk' & ts' & vi' & un' & ca' & hc' & hk' & hb' & ha' & hs & hm).
       eapply IH in hm; eauto.
-      + eapply step_meas_lt with (ca := ca); eauto.
-      + eapply step_preserves_stacks_wf_invar with (ca := ca); eauto.
+      + eapply step_parser_meas_lt; eauto.  
+      + eapply step_preserves_stack_wf_invar; eauto.
   Qed.
 
   Lemma parse_never_reaches_invalid_state :
-    forall (g  : grammar)
-           (x  : nonterminal)
-           (ts : list token),
-      parse g x ts <> Error InvalidState.
+    forall (gr  : grammar)
+           (hw  : grammar_wf gr)
+           (x   : nonterminal)
+           (ts  : list token),
+      parse gr hw x ts <> Error _ InvalidState.
   Proof.
-    intros g x ts hp; unfold parse in hp.
+    intros g hw x ts hp; unfold parse in hp.
     eapply multistep_never_reaches_error_state in hp; eauto.
     - apply lex_nat_triple_wf.
-    - eapply mkProductionMap_correct.
     - constructor.
   Qed.
 
@@ -87,49 +90,19 @@ Module ParserErrorFreeFn (Import D : Defs.T).
    when given a non-left-recursive grammar *)
   Lemma unavailable_nts_invar_starts_true :
     forall g x,
-      unavailable_nts_are_open_calls g NtSet.empty (SF None [x], []). 
+      unavailable_nts_are_open_calls g NtSet.empty (Fr [] tt [NT x], []). 
   Proof.
     intros g x; intros x' hi hni; ND.fsetdec.
   Qed.
 
-  (* to do : There is some redundancy here with proofs about
-   unavailable_nts_invar in Prediction. Those proofs should
-   be defined in terms of unavailable_nts_are_open_calls *)
-
-  Lemma return_preserves_unavailable_nts_invar :
-    forall g s_ce s_cr s_cr' s_frs o o' x suf vi,
-      s_ce     = SF o' []
-      -> s_cr  = SF o (NT x :: suf)
-      -> s_cr' = SF o suf
-      -> unavailable_nts_are_open_calls g vi (s_ce, s_cr :: s_frs)
-      -> unavailable_nts_are_open_calls g (NtSet.remove x vi) (s_cr', s_frs).
-  Proof.
-    intros; subst.
-    pose proof return_preserves_unavailable_nts_invar as hr; sis.
-    eapply hr; eauto.
-  Qed.
-
-  Lemma push_preserves_unavailable_nts_invar :
-    forall g s_cr s_ce s_frs vi o x suf rhs,
-      s_cr = SF o (NT x :: suf)
-      -> s_ce = SF (Some x) rhs
-      -> In (x, rhs) g
-      -> unavailable_nts_are_open_calls g vi (s_cr, s_frs)
-      -> unavailable_nts_are_open_calls g (NtSet.add x vi) (s_ce, s_cr :: s_frs).
-  Proof.
-    intros; subst.
-    pose proof push_preserves_unavailable_nts_invar as hp; sis.
-    eapply hp; eauto.
-  Qed.  
-
   Lemma step_preserves_unavailable_nts_invar :
-    forall g pm cm ps ps' ss ss' ts ts' vi vi' un un' ca ca' hc hk,
-      production_map_correct pm g
-      -> step pm cm ps ss ts vi un ca hc hk = StepK ps' ss' ts' vi' un' ca'
-      -> unavailable_nts_are_open_calls g vi  ss
-      -> unavailable_nts_are_open_calls g vi' ss'.
+    forall gr hw rm cm sk sk' ts ts' vi vi' un un' ca ca' hc hk,
+      rhs_map_correct rm gr
+      -> step gr hw rm cm sk ts vi un ca hc hk = StepK sk' ts' vi' un' ca'
+      -> unavailable_nts_are_open_calls gr vi  sk
+      -> unavailable_nts_are_open_calls gr vi' sk'.
   Proof.
-    intros g pm cm ps ps' ss ss' ts ts' vi vi' un un' ca ca' hc hk hp hs hu.
+    intros gr hw rm cm sk sk' ts ts' vi vi' un un' ca ca' hc hk hr hs hu.
     unfold step in hs; dmeqs h; tc; inv hs.
     - eapply return_preserves_unavailable_nts_invar; eauto. 
     - intros x hi hn; ND.fsetdec. 
@@ -137,144 +110,149 @@ Module ParserErrorFreeFn (Import D : Defs.T).
       eapply adaptivePredict_succ_in_grammar; eauto.
     - eapply push_preserves_unavailable_nts_invar; eauto.
       eapply adaptivePredict_ambig_in_grammar; eauto.
+      Unshelve.
+      all : auto.
   Qed.
 
   Lemma step_left_recursion_detection_sound :
-    forall g pm cm ps ss ts vi un ca hc hk x,
-      production_map_correct pm g
-      -> unavailable_nts_are_open_calls g vi ss
-      -> step pm cm ps ss ts vi un ca hc hk = StepError (LeftRecursion x)
-      -> left_recursive g (NT x).
+    forall gr hw rm cm sk ts vi un ca hc hk x,
+      rhs_map_correct rm gr
+      -> unavailable_nts_are_open_calls gr vi sk
+      -> step gr hw rm cm sk ts vi un ca hc hk = StepError (LeftRecursion x)
+      -> left_recursive gr (NT x).
   Proof.
-    intros g pm cm ps ss ts vi un ca hc hk x hp hu hs.
+    intros g hw rm cm sk ts vi un ca hc hk x hp hu hs.
     apply step_LeftRecursion_facts in hs.
-    destruct hs as [hi [[yss hf] [o [suf [frs heq]]]]]; subst.
+    destruct hs as [hi [[yss hf] [pre [vs [suf [frs heq]]]]]]; subst.
     apply hu in hi; auto.
-    - destruct hi as (frs_pre & cr & frs_suf & o' & suf' & ? & ? & hf'); subst.
+    - destruct hi as (frs_pre & cr & frs_suf & pre' & vs' & suf' & ? & ? & hf'); subst.
       eapply frnp_grammar_nullable_path; eauto.
     - eapply find_allNts; eauto.
   Qed.
 
   Lemma multistep_left_recursion_detection_sound :
-    forall (g      : grammar)
-           (pm     : production_map)
+    forall (gr     : grammar)
+           (hw     : grammar_wf gr)
+           (rm     : rhs_map)
+           (hr     : rhs_map_correct rm gr)
            (cm     : closure_map)
+           (x      : nonterminal)
            (tri    : nat * nat * nat)
            (ha     : Acc lex_nat_triple tri)
-           (ps     : prefix_stack)
-           (ss     : suffix_stack)
+           (sk     : parser_stack)
            (ts     : list token)
            (vi     : NtSet.t)
            (un     : bool)
            (ca     : cache)
-           (hc     : cache_stores_target_results pm cm ca)
-           (hk     : stack_pushes_from_keyset pm ss)
-           (ha'    : Acc lex_nat_triple (meas pm ss ts vi))
-           (x      : nonterminal),
-      tri = meas pm ss ts vi
-      -> production_map_correct pm g
-      -> unavailable_nts_are_open_calls g vi ss
-      -> multistep pm cm ps ss ts vi un ca hc hk ha' = Error (LeftRecursion x)
-      -> left_recursive g (NT x).
+           (hc     : cache_stores_target_results rm cm ca)
+           (hk     : stack_pushes_from_keyset rm sk)
+           (hb     : bottom_stack_sym_eq_start_sym sk x)
+           (ha'    : Acc lex_nat_triple (parser_meas rm sk ts vi))
+           (y      : nonterminal),
+      tri = parser_meas rm sk ts vi
+      -> unavailable_nts_are_open_calls gr vi sk
+      -> multistep gr hw rm hr cm x sk ts vi un ca hc hk hb ha' = Error _ (LeftRecursion y)
+      -> left_recursive gr (NT y).
   Proof.
-    intros g pm cm tri ha'; induction ha' as [tri hlt IH].
-    intros ps ss ts vi un ca hc hk ha x ? hp hu hm; subst.
+    intros gr hw rm hr cm x tri ha'; induction ha' as [tri hlt IH].
+    intros sk ts vi un ca hc hk hb ha y ? hu hm; subst.
     apply multistep_cases in hm.
     destruct hm as [hs | hm].
     - eapply step_left_recursion_detection_sound; eauto. 
-    - destruct hm as (ps' & ss' & ts' & vi' & un' & ca' & hc' & hk' & ha' & hs & hm).
-      eapply IH with (y := meas pm ss' ts' vi'); eauto.
-      + eapply step_meas_lt with (ca := ca); eauto.
-      + eapply step_preserves_unavailable_nts_invar with (ca := ca); eauto.
+    - destruct hm as (sk' & ts' & vi' & un' & ca' & hc' & hk' & hb' & ha' & hs & hm).
+      eapply IH with (y := parser_meas rm sk' ts' vi'); eauto.
+      + eapply step_parser_meas_lt; eauto. 
+      + eapply step_preserves_unavailable_nts_invar; eauto. 
   Qed.
 
   Lemma parse_left_recursion_detection_sound :
-    forall g x y ts,
-      parse g x ts = Error (LeftRecursion y)
-      -> left_recursive g (NT y).
+    forall gr hw x y ts,
+      parse gr hw x ts = Error _ (LeftRecursion y)
+      -> left_recursive gr (NT y).
   Proof.
-    intros g x y ts hp; unfold parse in hp.
+    intros g hw x y ts hp; unfold parse in hp.
     eapply multistep_left_recursion_detection_sound in hp; eauto.
     - apply lex_nat_triple_wf.
-    - apply mkProductionMap_correct.
     - intros x' hi hn; ND.fsetdec.
   Qed.
   
   Lemma parse_doesn't_find_left_recursion_in_non_left_recursive_grammar :
     forall (g   : grammar)
+           (hw  : grammar_wf g)
            (x y : nonterminal)
            (ts  : list token),
       no_left_recursion g
-      -> parse g x ts <> Error (LeftRecursion y).
+      -> parse g hw x ts <> Error _ (LeftRecursion y).
   Proof.
-    intros g x y ts hn hp.
+    intros g hw x y ts hn hp.
     apply parse_left_recursion_detection_sound in hp; firstorder.
   Qed.
 
   (* Errors never arise during prediction, given a non-left-recursive grammar *)
 
   Lemma step_never_returns_prediction_error :
-    forall g pm cm ps ss ts vi un ca hc hk e,
-      no_left_recursion g
-      -> production_map_correct pm g
-      -> closure_map_correct g cm
-      -> stacks_wf g ps ss
-      -> step pm cm ps ss ts vi un ca hc hk <> StepError (PredictionError e).
+    forall gr hw rm cm sk ts vi un ca hc hk e,
+      no_left_recursion gr
+      -> rhs_map_correct rm gr
+      -> closure_map_correct gr cm
+      -> stack_wf gr sk
+      -> step gr hw rm cm sk ts vi un ca hc hk <> StepError (PredictionError e).
   Proof.
-    intros g pm cm ps ss ts vi un ca hc hk e hn hp hm hw hs.
+    intros gr hw rm cm sk ts vi un ca hc hk e hn hp hm hw' hs.
     unfold step in hs; repeat dmeq h; tc; inv hs; sis; subst.
     eapply adaptivePredict_neq_error; eauto.
-    eapply frames_wf__suffix_frames_wf; eauto.
   Qed.
   
   Lemma multistep_never_returns_prediction_error :
-    forall (g      : grammar)
-           (pm     : production_map)
+    forall (gr     : grammar)
+           (hw     : grammar_wf gr)
+           (rm     : rhs_map)
+           (hr     : rhs_map_correct rm gr)
            (cm     : closure_map)
+           (x      : nonterminal)
            (tri    : nat * nat * nat)
            (a      : Acc lex_nat_triple tri)
-           (ps     : prefix_stack)
-           (ss     : suffix_stack)
+           (sk     : parser_stack)
            (ts     : list token)
            (vi     : NtSet.t)
            (un     : bool)
            (ca     : cache)
-           (hc     : cache_stores_target_results pm cm ca)
-           (hk     : stack_pushes_from_keyset pm ss)
-           (a'     : Acc lex_nat_triple (meas pm ss ts vi))
+           (hc     : cache_stores_target_results rm cm ca)
+           (hk     : stack_pushes_from_keyset rm sk)
+           (hb     : bottom_stack_sym_eq_start_sym sk x)
+           (a'     : Acc lex_nat_triple (parser_meas rm sk ts vi))
            (e      : prediction_error),
-      no_left_recursion g
-      -> production_map_correct pm g
-      -> closure_map_correct g cm 
-      -> tri = meas pm ss ts vi
-      -> stacks_wf g ps ss
-      -> multistep pm cm ps ss ts vi un ca hc hk a' <> Error (PredictionError e).
+      no_left_recursion gr
+      -> closure_map_correct gr cm 
+      -> tri = parser_meas rm sk ts vi
+      -> stack_wf gr sk
+      -> multistep gr hw rm hr cm x sk ts vi un ca hc hk hb a' <> Error _ (PredictionError e).
   Proof.
-    intros g pm cm tri a.
-    induction a as [tri hlt IH].
-    intros ps ss ts vi un ca hc hk a' e hn hp hcm ? hw hm; subst.
+    intros gr hw rm hr cm x tri ha.
+    induction ha as [tri hlt IH].
+    intros sk ts vi un ca hc hk hb ha' e hn hcm ? hw' hm; subst.
     apply multistep_cases in hm.
     destruct hm as [hs | hm].
     - eapply step_never_returns_prediction_error in hs; eauto.
-    - destruct hm as (ps' & ss' & ts' & av' & un' & ca' & hc' & hk' & a'' & hs & hm). 
+    - destruct hm as (sk' & ts' & av' & un' & ca' & hc' & hk' & hb' & a'' & hs & hm). 
       eapply IH in hm; eauto.
-      + eapply step_meas_lt with (ca := ca); eauto.
-      + eapply step_preserves_stacks_wf_invar with (ca := ca); eauto.
+      + eapply step_parser_meas_lt; eauto. 
+      + eapply step_preserves_stack_wf_invar; eauto. 
   Qed.
 
   Lemma parse_never_returns_prediction_error :
-    forall (g  : grammar)
-           (x  : nonterminal)
-           (ts : list token)
-           (e  : prediction_error),
-      no_left_recursion g
-      -> parse g x ts <> Error (PredictionError e).
+    forall (gr  : grammar)
+           (hw  : grammar_wf gr)
+           (x   : nonterminal)
+           (ts  : list token)
+           (e   : prediction_error),
+      no_left_recursion gr
+      -> parse gr hw x ts <> Error _ (PredictionError e).
   Proof.
-    intros g x ts e hn hp; unfold parse in hp.
+    intros g hw x ts e hn hp; unfold parse in hp.
     eapply multistep_never_returns_prediction_error in hp; eauto.
     - apply lex_nat_triple_wf.
-    - apply mkProductionMap_correct.
-    - apply mkClosureMap_result_correct.
+    - apply mkClosureMap_correct.
     - constructor.
   Qed.
 
